exercises/NoninterferenceTest.v
@@ -1,0 +1,202 @@
+Set Warnings "-notation-overridden,-parsing".
+From Coq Require Export String.
+From PLF Require Import Noninterference.
+
+Parameter MISSING: Type.
+
+Module Check.
+
+Ltac check_type A B :=
+    match type of A with
+    | context[MISSING] => idtac "Missing:" A
+    | ?T => first [unify T B; idtac "Type: ok" | idtac "Type: wrong - should be (" B ")"]
+    end.
+
+Ltac print_manual_grade A :=
+    match eval compute in A with
+    | Some (_ ?S ?C) =>
+        idtac "Score:"  S;
+        match eval compute in C with
+          | ""%string => idtac "Comment: None"
+          | _ => idtac "Comment:" C
+        end
+    | None =>
+        idtac "Score: Ungraded";
+        idtac "Comment: None"
+    end.
+
+End Check.
+
+From PLF Require Import Noninterference.
+Import Check.
+
+Goal True.
+
+idtac "-------------------  prove_or_disprove_obvious_f1  --------------------".
+idtac " ".
+
+idtac "#> prove_or_disprove_obvious_f1".
+idtac "Possible points: 1".
+check_type @prove_or_disprove_obvious_f1 (
+(@noninterferent nat nat nat nat obvious_f1 \/
+ ~ @noninterferent nat nat nat nat obvious_f1)).
+idtac "Assumptions:".
+Abort.
+Print Assumptions prove_or_disprove_obvious_f1.
+Goal True.
+idtac " ".
+
+idtac "-------------------  prove_or_disprove_obvious_f2  --------------------".
+idtac " ".
+
+idtac "#> prove_or_disprove_obvious_f2".
+idtac "Possible points: 1".
+check_type @prove_or_disprove_obvious_f2 (
+(@noninterferent nat nat nat nat obvious_f2 \/
+ ~ @noninterferent nat nat nat nat obvious_f2)).
+idtac "Assumptions:".
+Abort.
+Print Assumptions prove_or_disprove_obvious_f2.
+Goal True.
+idtac " ".
+
+idtac "-------------------  prove_or_disprove_less_obvious_f4  --------------------".
+idtac " ".
+
+idtac "#> prove_or_disprove_less_obvious_f4".
+idtac "Possible points: 2".
+check_type @prove_or_disprove_less_obvious_f4 (
+(@noninterferent nat nat nat nat less_obvious_f4 \/
+ ~ @noninterferent nat nat nat nat less_obvious_f4)).
+idtac "Assumptions:".
+Abort.
+Print Assumptions prove_or_disprove_less_obvious_f4.
+Goal True.
+idtac " ".
+
+idtac "-------------------  prove_or_disprove_less_obvious_f5  --------------------".
+idtac " ".
+
+idtac "#> prove_or_disprove_less_obvious_f5".
+idtac "Possible points: 2".
+check_type @prove_or_disprove_less_obvious_f5 (
+(@noninterferent nat nat nat nat less_obvious_f5 \/
+ ~ @noninterferent nat nat nat nat less_obvious_f5)).
+idtac "Assumptions:".
+Abort.
+Print Assumptions prove_or_disprove_less_obvious_f5.
+Goal True.
+idtac " ".
+
+idtac "-------------------  prove_or_disprove_less_obvious_f6  --------------------".
+idtac " ".
+
+idtac "#> prove_or_disprove_less_obvious_f6".
+idtac "Possible points: 2".
+check_type @prove_or_disprove_less_obvious_f6 (
+(@noninterferent nat nat nat nat less_obvious_f6 \/
+ ~ @noninterferent nat nat nat nat less_obvious_f6)).
+idtac "Assumptions:".
+Abort.
+Print Assumptions prove_or_disprove_less_obvious_f6.
+Goal True.
+idtac " ".
+
+idtac "-------------------  sme_another_insecure_f2  --------------------".
+idtac " ".
+
+idtac "#> sme_another_insecure_f2".
+idtac "Possible points: 1".
+check_type @sme_another_insecure_f2 (
+(forall pi si : nat,
+ @sme nat nat nat nat 0 another_insecure_f2 pi si = (pi, pi + si))).
+idtac "Assumptions:".
+Abort.
+Print Assumptions sme_another_insecure_f2.
+Goal True.
+idtac " ".
+
+idtac "-------------------  sme_another_insecure_f3  --------------------".
+idtac " ".
+
+idtac "#> sme_another_insecure_f3".
+idtac "Possible points: 2".
+check_type @sme_another_insecure_f3 (
+(forall pi si : nat,
+ @sme nat nat nat nat 0 another_insecure_f3 pi si = (pi, pi + si))).
+idtac "Assumptions:".
+Abort.
+Print Assumptions sme_another_insecure_f3.
+Goal True.
+idtac " ".
+
+idtac "-------------------  noninterferent_secure_com_exercise  --------------------".
+idtac " ".
+
+idtac "#> noninterferent_secure_com_exercise".
+idtac "Possible points: 2".
+check_type @noninterferent_secure_com_exercise (
+(noninterferent_no_while xpub secure_com_exercise)).
+idtac "Assumptions:".
+Abort.
+Print Assumptions noninterferent_secure_com_exercise.
+Goal True.
+idtac " ".
+
+idtac "-------------------  interferent_insecure_com_explicit  --------------------".
+idtac " ".
+
+idtac "#> interferent_insecure_com_explicit".
+idtac "Possible points: 2".
+check_type @interferent_insecure_com_explicit (
+(~ noninterferent_no_while xpub insecure_com_explicit)).
+idtac "Assumptions:".
+Abort.
+Print Assumptions interferent_insecure_com_explicit.
+Goal True.
+idtac " ".
+
+idtac " ".
+
+idtac "Max points - standard: 15".
+idtac "Max points - advanced: 15".
+idtac "".
+idtac "Allowed Axioms:".
+idtac "functional_extensionality".
+idtac "FunctionalExtensionality.functional_extensionality_dep".
+idtac "".
+idtac "".
+idtac "********** Summary **********".
+idtac "".
+idtac "Below is a summary of the automatically graded exercises that are incomplete.".
+idtac "".
+idtac "The output for each exercise can be any of the following:".
+idtac "  - 'Closed under the global context', if it is complete".
+idtac "  - 'MANUAL', if it is manually graded".
+idtac "  - A list of pending axioms, containing unproven assumptions. In this case".
+idtac "    the exercise is considered complete, if the axioms are all allowed.".
+idtac "".
+idtac "********** Standard **********".
+idtac "---------- prove_or_disprove_obvious_f1 ---------".
+Print Assumptions prove_or_disprove_obvious_f1.
+idtac "---------- prove_or_disprove_obvious_f2 ---------".
+Print Assumptions prove_or_disprove_obvious_f2.
+idtac "---------- prove_or_disprove_less_obvious_f4 ---------".
+Print Assumptions prove_or_disprove_less_obvious_f4.
+idtac "---------- prove_or_disprove_less_obvious_f5 ---------".
+Print Assumptions prove_or_disprove_less_obvious_f5.
+idtac "---------- prove_or_disprove_less_obvious_f6 ---------".
+Print Assumptions prove_or_disprove_less_obvious_f6.
+idtac "---------- sme_another_insecure_f2 ---------".
+Print Assumptions sme_another_insecure_f2.
+idtac "---------- sme_another_insecure_f3 ---------".
+Print Assumptions sme_another_insecure_f3.
+idtac "---------- noninterferent_secure_com_exercise ---------".
+Print Assumptions noninterferent_secure_com_exercise.
+idtac "---------- interferent_insecure_com_explicit ---------".
+Print Assumptions interferent_insecure_com_explicit.
+idtac "".
+idtac "********** Advanced **********".
+Abort.
+
+(* 2025-05-28 23:56 *)
